refactor: remove useless parameter of YjsLt (#3)
* refactor: remove useless parameter of YjsLt

* fix errors

* fix: remove sorry

* fix: remove non related code

LeanYjs/ItemOrder.lean
@@ -22,45 +22,45 @@ inductive OriginReachable {A} : YjsPtr A -> YjsPtr A -> Prop where
   | reachable_head : forall x y z, OriginReachableStep x y -> OriginReachable y z -> OriginReachable x z
 
 mutual
-  inductive YjsLt {A : Type} (P : ItemSet A) : Nat -> YjsPtr A -> YjsPtr A -> Prop where
-    | ltConflict h i1 i2 : ConflictLt P h i1 i2 -> YjsLt P (h + 1) i1 i2
-    | ltOriginOrder i1 i2 : P i1 -> P i2 -> OriginLt i1 i2 -> YjsLt P 0 i1 i2
-    | ltOrigin h x o r id c : P (YjsItem.item o r id c) -> YjsLeq P h x o -> YjsLt P (h + 1) x (YjsItem.item o r id c)
-    | ltRightOrigin h o r id c x : P (YjsItem.item o r id c) -> YjsLeq P h r x -> YjsLt P (h + 1) (YjsItem.item o r id c) x
+  inductive YjsLt {A : Type} : Nat -> YjsPtr A -> YjsPtr A -> Prop where
+    | ltConflict h i1 i2 : ConflictLt h i1 i2 -> YjsLt (h + 1) i1 i2
+    | ltOriginOrder i1 i2 : OriginLt i1 i2 -> YjsLt 0 i1 i2
+    | ltOrigin h x o r id c : YjsLeq h x o -> YjsLt (h + 1) x (YjsItem.item o r id c)
+    | ltRightOrigin h o r id c x : YjsLeq h r x -> YjsLt (h + 1) (YjsItem.item o r id c) x
 
-  inductive YjsLeq {A : Type} (P : ItemSet A) : Nat -> YjsPtr A -> YjsPtr A -> Prop where
-    | leqSame x : P x -> YjsLeq P h x x
-    | leqLt h x y : YjsLt P h x y -> YjsLeq P (h + 1) x y
+  inductive YjsLeq {A : Type} : Nat -> YjsPtr A -> YjsPtr A -> Prop where
+    | leqSame x : YjsLeq h x x
+    | leqLt h x y : YjsLt h x y -> YjsLeq (h + 1) x y
 
-  inductive ConflictLt {A : Type} (P : ItemSet A) : Nat -> YjsPtr A -> YjsPtr A -> Prop where
+  inductive ConflictLt {A : Type} : Nat -> YjsPtr A -> YjsPtr A -> Prop where
     | ltOriginDiff h1 h2 h3 h4 l1 l2 r1 r2 id1 id2 c1 c2 :
-      YjsLt P h1 l2 l1
-      -> YjsLt P h2 (YjsItem.item l1 r1 id1 c1) r2
-      -> YjsLt P h3 l1 (YjsItem.item l2 r2 id2 c2)
-      -> YjsLt P h4 (YjsItem.item l2 r2 id2 c2) r1
-      -> ConflictLt P (max4 h1 h2 h3 h4 + 1) (YjsItem.item l1 r1 id1 c1) (YjsItem.item l2 r2 id2 c2)
+      YjsLt h1 l2 l1
+      -> YjsLt h2 (YjsItem.item l1 r1 id1 c1) r2
+      -> YjsLt h3 l1 (YjsItem.item l2 r2 id2 c2)
+      -> YjsLt h4 (YjsItem.item l2 r2 id2 c2) r1
+      -> ConflictLt (max4 h1 h2 h3 h4 + 1) (YjsItem.item l1 r1 id1 c1) (YjsItem.item l2 r2 id2 c2)
     | ltOriginSame h1 h2 l r1 r2 id1 id2 (c1 c2 : A) :
-      YjsLt P h1 (YjsItem.item l r1 id1 c1) r2
-      -> YjsLt P h2 (YjsItem.item l r2 id2 c2) r1
+      YjsLt h1 (YjsItem.item l r1 id1 c1) r2
+      -> YjsLt h2 (YjsItem.item l r2 id2 c2) r1
       -> id1 < id2
-      -> ConflictLt P (max h1 h2 + 1) (YjsItem.item l r1 id1 c1) (YjsItem.item l r2 id2 c2)
+      -> ConflictLt (max h1 h2 + 1) (YjsItem.item l r1 id1 c1) (YjsItem.item l r2 id2 c2)
 end
 
-def ConflictLt' {A} (P : ItemSet A) (i1 i2 : YjsPtr A) : Prop :=
-  ∃ h, ConflictLt P h i1 i2
+def ConflictLt' {A} (i1 i2 : YjsPtr A) : Prop :=
+  ∃ h, ConflictLt h i1 i2
 
-def YjsLt' {A} (P : ItemSet A) (x y : YjsPtr A) : Prop :=
-  ∃ h, @YjsLt A P h x y
+def YjsLt' {A} (x y : YjsPtr A) : Prop :=
+  ∃ h, @YjsLt A h x y
 
-def YjsLeq' {A} (P : ItemSet A) (x y : YjsPtr A) : Prop :=
-  ∃ h, @YjsLeq A P h x y
+def YjsLeq' {A} (x y : YjsPtr A) : Prop :=
+  ∃ h, @YjsLeq A h x y
 
-theorem ConflictLt'.ltOriginDiff {A : Type} (P : ItemSet A) l1 l2 r1 r2 id1 id2 c1 c2 :
-  YjsLt' P l2 l1
-  -> YjsLt' P (YjsItem.item l1 r1 id1 c1) r2
-  -> YjsLt' P l1 (YjsItem.item l2 r2 id2 c2)
-  -> YjsLt' P (YjsItem.item l2 r2 id2 c2) r1
-  -> ConflictLt' P (YjsItem.item l1 r1 id1 c1) (YjsItem.item l2 r2 id2 c2) := by
+theorem ConflictLt'.ltOriginDiff {A : Type} (l1 l2 r1 r2 : YjsPtr A) (id1 id2 : ClientId) (c1 c2 : A) :
+  YjsLt' l2 l1
+  -> YjsLt' (YjsItem.item l1 r1 id1 c1) r2
+  -> YjsLt' l1 (YjsItem.item l2 r2 id2 c2)
+  -> YjsLt' (YjsItem.item l2 r2 id2 c2) r1
+  -> ConflictLt' (A := A) (YjsItem.item l1 r1 id1 c1) (YjsItem.item l2 r2 id2 c2) := by
   intros hlt1 hlt2 hlt3 hlt4
   obtain ⟨ h1, hlt1 ⟩ := hlt1
   obtain ⟨ h2, hlt2 ⟩ := hlt2
@@ -69,220 +69,73 @@ theorem ConflictLt'.ltOriginDiff {A : Type} (P : ItemSet A) l1 l2 r1 r2 id1 id2 
   constructor
   apply ConflictLt.ltOriginDiff <;> try assumption
 
-theorem ConflictLt'.ltOriginSame {A : Type} (P : ItemSet A) l r1 r2 id1 id2 c1 c2 :
-  YjsLt' P (YjsItem.item l r1 id1 c1) r2
-  -> YjsLt' P (YjsItem.item l r2 id2 c2) r1
+theorem ConflictLt'.ltOriginSame {A : Type} (l r1 r2 : YjsPtr A) (id1 id2 : ClientId) (c1 c2 : A) :
+  YjsLt' (YjsItem.item l r1 id1 c1) r2
+  -> YjsLt' (YjsItem.item l r2 id2 c2) r1
   -> id1 < id2
-  -> ConflictLt' P (YjsItem.item l r1 id1 c1) (YjsItem.item l r2 id2 c2) := by
+  -> ConflictLt' (A := A) (YjsItem.item l r1 id1 c1) (YjsItem.item l r2 id2 c2) := by
   intros hlt1 hlt2 hlt3
   obtain ⟨ h1, hlt1 ⟩ := hlt1
   obtain ⟨ h2, hlt2 ⟩ := hlt2
   constructor
   apply ConflictLt.ltOriginSame <;> try assumption
 
-theorem YjsLt'.ltConflict {A : Type} (P : ItemSet A) i1 i2 : ConflictLt' P i1 i2 -> YjsLt' P i1 i2 := by
+theorem YjsLt'.ltConflict {A : Type} (i1 i2 : YjsPtr A) : ConflictLt' i1 i2 -> YjsLt' i1 i2 := by
   intros hlt
   obtain ⟨ h, hlt ⟩ := hlt
   constructor
   apply YjsLt.ltConflict
   assumption
 
-theorem YjsLt'.ltOriginOrder {A : Type} (P : ItemSet A) i1 i2 : P i1 -> P i2 -> OriginLt i1 i2 -> YjsLt' P i1 i2 := by
-  intros hpi1 hpi2 hor
+theorem YjsLt'.ltOriginOrder {A : Type} (i1 i2 : YjsPtr A) : OriginLt i1 i2 -> YjsLt' i1 i2 := by
+  intros hor
   constructor
-  apply YjsLt.ltOriginOrder <;> try assumption
+  apply YjsLt.ltOriginOrder; assumption
 
-theorem YjsLt'.ltOrigin {A : Type} (P : ItemSet A) x o r id c : P (YjsItem.item o r id c) -> YjsLeq' P x o -> YjsLt' P x (YjsItem.item o r id c) := by
-  intros hpi hleq
+theorem YjsLt'.ltOrigin {A : Type} (x o r : YjsPtr A) id c : YjsLeq' x o -> YjsLt' x (YjsItem.item o r id c) := by
+  intros hleq
   obtain ⟨ h, hleq ⟩ := hleq
   constructor
   apply YjsLt.ltOrigin <;> try assumption
 
-theorem YjsLt'.ltRightOrigin {A : Type} (P : ItemSet A) o r id c x : P (YjsItem.item o r id c) -> YjsLeq' P r x -> YjsLt' P (YjsItem.item o r id c) x := by
-  intros hpi hleq
+theorem YjsLt'.ltRightOrigin {A : Type} (o r : YjsPtr A) id c x : YjsLeq' r x -> YjsLt' (YjsItem.item o r id c) x := by
+  intros hleq
   obtain ⟨ h, hleq ⟩ := hleq
   constructor
   apply YjsLt.ltRightOrigin <;> try assumption
 
-theorem YjsLeq'.leqSame {A : Type} (P : ItemSet A) x : P x -> YjsLeq' P x x := by
-  intros hpx
+theorem YjsLeq'.leqSame {A : Type} (x : YjsPtr A) : YjsLeq' x x := by
   exists 0
   apply YjsLeq.leqSame
-  assumption
 
-theorem YjsLeq'.leqLt {A : Type} (P : ItemSet A) x y : YjsLt' P x y -> YjsLeq' P x y := by
+theorem YjsLeq'.leqLt {A : Type} (x y : YjsPtr A) : YjsLt' x y -> YjsLeq' x y := by
   intros hlt
   obtain ⟨ h, hlt ⟩ := hlt
   exists h + 1
   apply YjsLeq.leqLt
   assumption
 
-theorem yjs_lt_p1_aux {A : Type} {P : @ItemSet A} {h : Nat} : forall {x y : YjsPtr A},
-  (YjsLt P h x y -> P x) ∧ (ConflictLt P h x y -> P x) ∧ (YjsLeq P h x y -> P x) := by
-    apply Nat.strongRecOn' (P := fun h => ∀ x y, (YjsLt P h x y -> P x) ∧ (ConflictLt P h x y -> P x) ∧ (YjsLeq P h x y -> P x))
-    intros n ih x y
-    constructor
-    . intro hlt
-      cases hlt with
-      | ltConflict h x y hlt =>
-        have hlt_h : h < h + 1 := by
-          omega
-        let ⟨ _, h, _ ⟩ := ih h hlt_h x y
-        apply h ; assumption
-      | ltOriginOrder x y _ =>
-        assumption
-      | ltOrigin h x o r id c hval hlt =>
-        have hlt_h : h < h + 1 := by
-          omega
-        let ⟨ _, _, ih ⟩ := ih h hlt_h x o
-        apply ih; assumption
-      | ltRightOrigin h o r id c x hval hlt =>
-        assumption
-    . constructor
-      . intro hlt
-        cases hlt with
-        | ltOriginDiff h1 h2 h3 h4 l1 l2 r1 r2 id1 id2 c1 c2 hlt1 hlt2 hlt3 =>
-          have hlt_h : h2 < max4 h1 h2 h3 h4 + 1 := by
-            unfold max4
-            omega
-          let ⟨ ih, _ ⟩ := ih h2 hlt_h (YjsPtr.itemPtr (YjsItem.item l1 r1 id1 c1)) r2
-          apply ih hlt2
-        | ltOriginSame h1 h2 l r1 r2 id1 id2 c1 c2 hlt1 hlt2 _ =>
-          have hlt_h : h1 < max h1 h2 + 1 := by
-            omega
-          let ⟨ ih, _ ⟩ := ih h1 hlt_h (YjsPtr.itemPtr (YjsItem.item l r1 id1 c1)) r2
-          apply ih hlt1
-      . intros hlt
-        cases hlt with
-        | leqSame hpx x =>
-          assumption
-        | leqLt h x y hlt =>
-          obtain ⟨ ih, _, _ ⟩ := ih h (by omega) x y
-          apply ih; assumption
-
-@[simp] theorem yjs_lt_p1 {A : Type} {P : @ItemSet A} {h : Nat} : forall {x y : YjsPtr A},
-  YjsLt P h x y -> P x := by
-    intros x y hlt
-    let ⟨ h, _ ⟩ := @yjs_lt_p1_aux A P h x y
-    tauto
-
-theorem yjs_lt'_p1 {A : Type} {P : @ItemSet A} : forall {x y : YjsPtr A},
-  YjsLt' P x y -> P x := by
-    intros x y hlt
-    obtain ⟨ h, hlt ⟩ := hlt
-    apply yjs_lt_p1; assumption
-
-theorem conflict_lt_p1 {A : Type} {P : @ItemSet A} {h : Nat} : forall {x y : YjsPtr A},
-  ConflictLt P h x y -> P x := by
-    intros x y hlt
-    let ⟨ _, h ⟩ := @yjs_lt_p1_aux A P h x y
-    tauto
-
-theorem yjs_lt_p2_aux {A : Type} {P : @ItemSet A} {h : Nat} : forall {x y : YjsPtr A},
-  (YjsLt P h x y -> P y) ∧ (ConflictLt P h x y -> P y) ∧ (YjsLeq P h x y -> P y) := by
-    apply Nat.strongRecOn' (P := fun h => ∀ x y, (YjsLt P h x y -> P y) ∧ (ConflictLt P h x y -> P y) ∧ (YjsLeq P h x y -> P y))
-    intros n ih x y
-    constructor
-    . intro hlt
-      cases hlt with
-      | ltConflict h x y hlt =>
-        have hlt_h : h < h + 1 := by
-          omega
-        let ⟨ _, h, _ ⟩ := ih h hlt_h x y
-        apply h ; assumption
-      | ltOriginOrder x y _ =>
-        assumption
-      | ltOrigin h x o r id c hval hlt =>
-        assumption
-      | ltRightOrigin h o r id c x hval hlt =>
-        have hlt_h : h < h + 1 := by
-          omega
-        let ⟨ _, _, ih ⟩ := ih h hlt_h r y
-        apply ih; assumption
-    . constructor
-      . intro hlt
-        cases hlt with
-        | ltOriginDiff h1 h2 h3 h4 l1 l2 r1 r2 id1 id2 c1 c2 hlt1 hlt2 hlt3 =>
-          have hlt_h : h3 < max4 h1 h2 h3 h4 + 1 := by
-            unfold max4
-            omega
-          let ⟨ ih, _ ⟩ := ih h3 hlt_h l1 (YjsPtr.itemPtr (YjsItem.item l2 r2 id2 c2))
-          apply ih hlt3
-        | ltOriginSame h1 h2 l r1 r2 id1 id2 c1 c2 hlt1 hlt2 _ =>
-          apply yjs_lt_p1; assumption
-      . intros hlt
-        cases hlt with
-        | leqSame hpx x =>
-          assumption
-        | leqLt h x y hlt =>
-          obtain ⟨ ih, _, _ ⟩ := ih h (by omega) x y
-          apply ih; assumption
-
-theorem yjs_lt_p2 {A : Type} {P : @ItemSet A} {h : Nat} : forall {x y : YjsPtr A},
-  YjsLt P h x y -> P y := by
-    intros x y hlt
-    let ⟨ h, _ ⟩ := @yjs_lt_p2_aux A P h x y
-    tauto
-
-theorem yjs_lt'_p2 {A : Type} {P : @ItemSet A} : forall {x y : YjsPtr A},
-  YjsLt' P x y -> P y := by
-    intros x y hlt
-    obtain ⟨ h, hlt ⟩ := hlt
-    apply yjs_lt_p2; assumption
-
-theorem conflict_lt_p2 {A : Type} {P : @ItemSet A} {h : Nat} : forall {x y : YjsPtr A},
-  ConflictLt P h x y -> P y := by
-    intros x y hlt
-    let ⟨ _, h ⟩ := @yjs_lt_p2_aux A P h x y
-    tauto
-
-theorem yjs_leq_p1 {A : Type} {P : @ItemSet A} {h : Nat} : forall {x y : YjsPtr A},
-  YjsLeq P h x y -> P y -> P x := by
-    intros x y hleq hpy
-    cases hleq with
-    | leqSame => assumption
-    | leqLt _ _ _  hlt => apply yjs_lt_p1 hlt
-
-theorem yjs_leq_p2 {A : Type} {P : @ItemSet A} {h : Nat} : forall {x y : YjsPtr A},
-  YjsLeq P h x y -> P x -> P y := by
-    intros x y hleq hpy
-    cases hleq with
-    | leqSame => assumption
-    | leqLt _ _ _ hlt => apply yjs_lt_p2 hlt
-
-def yjs_leq'_imp_eq_or_yjs_lt' {A : Type} {P : @ItemSet A} {x y : YjsPtr A} :
-  YjsLeq' P x y -> x = y ∨ YjsLt' P x y := by
+def yjs_leq'_imp_eq_or_yjs_lt' {A : Type} {x y : YjsPtr A} :
+  YjsLeq' x y -> x = y ∨ YjsLt' x y := by
     intros hleq
     obtain ⟨ h, hleq ⟩ := hleq
     cases hleq with
     | leqSame _ => left; rfl
     | leqLt _ _ _ hlt => right; constructor; assumption
 
-theorem yjs_leq'_p1 {A : Type} {P : @ItemSet A} : forall {x y : YjsPtr A},
-  YjsLeq' P x y -> P y -> P x := by
-    intros x y hleq hpy
-    obtain ⟨ h, hleq ⟩ := hleq
-    apply yjs_leq_p1 hleq hpy
-
-theorem yjs_leq'_p2 {A : Type} {P : @ItemSet A} : forall {x y : YjsPtr A},
-  YjsLeq' P x y -> P x -> P y := by
-    intros x y hleq hpy
-    obtain ⟨ h, hleq ⟩ := hleq
-    apply yjs_leq_p2 hleq hpy
-
-theorem yjs_lt_cases A P h (x y : YjsPtr A) :
-  YjsLt P h x y ->
+theorem yjs_lt_cases A h (x y : YjsPtr A) :
+  YjsLt h x y ->
     (x = YjsPtr.first ∧ (y = YjsPtr.last ∨ ∃ i, y = YjsPtr.itemPtr i)) ∨
     (y = YjsPtr.last ∧ (x = YjsPtr.first ∨ ∃ i, x = YjsPtr.itemPtr i)) ∨
-    (∃ x', x = YjsPtr.itemPtr x' ∧ YjsLeq' P x'.rightOrigin y) ∨
-    (∃ y', y = YjsPtr.itemPtr y' ∧ YjsLeq' P x y'.origin) ∨
-    ConflictLt' P x y := by
+    (∃ x', x = YjsPtr.itemPtr x' ∧ YjsLeq' x'.rightOrigin y) ∨
+    (∃ y', y = YjsPtr.itemPtr y' ∧ YjsLeq' x y'.origin) ∨
+    ConflictLt' x y := by
   intros hlt
   cases hlt with
   | ltConflict h x y hlt =>
     right; right; right; right
     apply Exists.intro h; assumption
-  | ltOriginOrder x y px py hlt =>
+  | ltOriginOrder x y hlt =>
     cases hlt with
     | lt_first_last =>
       left; simp
@@ -290,65 +143,20 @@ theorem yjs_lt_cases A P h (x y : YjsPtr A) :
       left; simp
     | lt_last =>
       right; left; simp
-  | ltOrigin h x o r id c hval hlt =>
+  | ltOrigin h x o r id c hlt =>
     right; right; right; left; simp
     constructor; assumption
-  | ltRightOrigin h o r id c x hval hlt =>
+  | ltRightOrigin h o r id c x hlt =>
     right; right; left; simp
     constructor; assumption
 
-theorem yjs_lt'_cases A P (x y : YjsPtr A) :
-  YjsLt' P x y ->
+theorem yjs_lt'_cases A (x y : YjsPtr A) :
+  YjsLt' x y ->
     (x = YjsPtr.first ∧ (y = YjsPtr.last ∨ ∃ i, y = YjsPtr.itemPtr i)) ∨
     (y = YjsPtr.last ∧ (x = YjsPtr.first ∨ ∃ i, x = YjsPtr.itemPtr i)) ∨
-    (∃ x', x = YjsPtr.itemPtr x' ∧ YjsLeq' P x'.rightOrigin y) ∨
-    (∃ y', y = YjsPtr.itemPtr y' ∧ YjsLeq' P x y'.origin) ∨
-    ConflictLt' P x y := by
+    (∃ x', x = YjsPtr.itemPtr x' ∧ YjsLeq' x'.rightOrigin y) ∨
+    (∃ y', y = YjsPtr.itemPtr y' ∧ YjsLeq' x y'.origin) ∨
+    ConflictLt' x y := by
   intros hlt
   obtain ⟨ h, hlt ⟩ := hlt
-  apply yjs_lt_cases A P h x y hlt
-
--- inductive LtSequence {A : Type} (P : @ItemSet A) : YjsPtr A -> YjsPtr A -> List (YjsPtr A) -> Prop where
---   | base : forall x, LtSequence P x x []
---   | step1 : forall x y z is h, ConflictLt P h x y -> LtSequence P y z is -> LtSequence P x z (y :: is)
---   | step2 : forall x y z is, OriginLt _ x y -> LtSequence P y z is -> LtSequence P x z (y :: is)
-
--- theorem LtSequenceConcat {A : Type} {P : @ItemSet A} {x y z : YjsPtr A} {is1 is2 : List (YjsPtr A)} :
---   LtSequence P x y is1 -> LtSequence P y z is2 -> LtSequence P x z (is1 ++ is2) := by
---     intro lt1
---     induction lt1 with
---     | base x =>
---       intros lt2
---       apply lt2
---     | step1 x y z is _ lt1 lt2 ih =>
---       intros lt
---       apply LtSequence.step1 <;> try assumption
---       apply ih
---       assumption
---     | step2 x y z is lt1 lt2 ih =>
---       intros lt
---       apply LtSequence.step2 <;> try assumption
---       apply ih
---       assumption
-
--- theorem YjsLtSequence (A : Type) (P : ItemSet A): forall (x y : YjsPtr A) h, YjsLt P h x y ->
---   ∃ is : List (YjsPtr A), LtSequence P x y is := by
---     intros x y h
---     apply Nat.strongRecOn' (P := fun h => ∀ x y, YjsLt P h x y -> ∃ is : List (YjsPtr A), LtSequence P x y is)
---     intros h' ih x y lt
---     match lt with
---     | YjsLt.ltConflict h x y _ =>
---       apply Exists.intro [y]
---       apply LtSequence.step1 <;> try assumption
---       apply LtSequence.base
---     | YjsLt.ltOriginOrder x y hx hy hlt =>
---       apply Exists.intro [y]
---       apply LtSequence.step2 <;> try assumption
---       apply LtSequence.base
---     | YjsLt.ltOrigin h x o r id c hval hlt =>
---       have hlt_h : h < h + 1 := by
---         omega
---       let ⟨ is, ih ⟩ := ih h hlt_h x o hlt
---       apply Exists.intro (is ++ [o])
---       apply LtSequenceConcat ih
---       apply LtSequence.step1
+  apply yjs_lt_cases A h x y hlt
