LeanYjs.lean
@@ -1,6 +1,6 @@
 -- This module serves as the root of the `LeanYjs` library.
 -- Import modules here that should be built as part of the library.
-import LeanYjs.ListExtra
+import LeanYjs.ListLemmas
 import LeanYjs.Item
 import LeanYjs.ItemSet
 import LeanYjs.ClientId
